end of day 19/04/20

inference-tool/src/main/scala/inference/Dirties.scala
@@ -160,11 +160,11 @@ object Dirties {
     val f = "intermediate_" + randomUUID.toString().replace("-", "_")
     TypeConversion.doubleEFSMToSALTranslator(Inference.tm(e1), "e1", Inference.tm(e2), "e2", f)
     addLTL(s"salfiles/${f}.sal", s"composition: MODULE = (RENAME o to o_e1 IN e1) || (RENAME o to o_e2 IN e2);\n" +
-      s"canTake: THEOREM composition |- G(cfstate.1 = ${TypeConversion.salState(s1)} AND cfstate.2 = ${TypeConversion.salState(s2)} => NOT(input_sequence ! size?(i) = ${Code_Numeral.integer_of_nat(Transition.Arity(t2))} AND ${efsm2sal.guards2sal(Transition.Guard(t2))}));")
+      s"canTake: THEOREM composition |- G(cfstate.1 = ${TypeConversion.salState(s1)} AND cfstate.2 = ${TypeConversion.salState(s2)} => NOT(input_sequence ! size?(i) = ${Code_Numeral.integer_of_nat(Transition.Arity(t2))} AND ${efsm2sal.guards2sal(Transition.Guards(t2))}));")
     val output = Seq("bash", "-c", s"cd salfiles; sal-smc --assertion='${f}{${maxNum(e1, e2)}}!canTake'").!!
     if (!output.toString.startsWith("Counterexample")) {
       Log.root.warn(s"""Path failure:\n
-      G(cfstate.1 = ${TypeConversion.salState(s1)} AND cfstate.2 = ${TypeConversion.salState(s2)} => NOT(input_sequence ! size?(I) = ${Code_Numeral.integer_of_nat(Transition.Arity(t2))} AND ${efsm2sal.guards2sal(Transition.Guard(t2))}));\n
+      G(cfstate.1 = ${TypeConversion.salState(s1)} AND cfstate.2 = ${TypeConversion.salState(s2)} => NOT(input_sequence ! size?(I) = ${Code_Numeral.integer_of_nat(Transition.Arity(t2))} AND ${efsm2sal.guards2sal(Transition.Guards(t2))}));\n
       sal-smc --assertion='${f}{${maxNum(e1, e2)}}!canTake'""")
     }
     FileUtils.deleteQuietly(new File(s"salfiles/${f}.sal"))
@@ -254,8 +254,8 @@ object Dirties {
           NOT(
             cfstate.1 = ${TypeConversion.salState(s1)} AND
             cfstate.2 = ${TypeConversion.salState(s2)} AND
-            input_sequence ! size?(i) = ${Code_Numeral.integer_of_nat(Transition.Arity(t1))} AND ${efsm2sal.guards2sal(Transition.Guard(t1))} AND
-            input_sequence ! size?(i) = ${Code_Numeral.integer_of_nat(Transition.Arity(t2))} AND ${efsm2sal.guards2sal(Transition.Guard(t2))} AND
+            input_sequence ! size?(i) = ${Code_Numeral.integer_of_nat(Transition.Arity(t1))} AND ${efsm2sal.guards2sal(Transition.Guards(t1))} AND
+            input_sequence ! size?(i) = ${Code_Numeral.integer_of_nat(Transition.Arity(t2))} AND ${efsm2sal.guards2sal(Transition.Guards(t2))} AND
             X(o_e1 /= o_e2)
           )
         );""")
@@ -282,8 +282,8 @@ object Dirties {
                 NOT(
                     cfstate.1 = ${TypeConversion.salState(s1)} =>
                     cfstate.2 = ${TypeConversion.salState(s2)} =>
-                    ((input_sequence ! size?(i) = ${Code_Numeral.integer_of_nat(Transition.Arity(t2))} AND ${efsm2sal.guards2sal_num(Transition.Guard(t2), Nat.Nata(2))}) =>
-                  (input_sequence ! size?(i) = ${Code_Numeral.integer_of_nat(Transition.Arity(t1))} AND ${efsm2sal.guards2sal_num(Transition.Guard(t1), Nat.Nata(1))}))
+                    ((input_sequence ! size?(i) = ${Code_Numeral.integer_of_nat(Transition.Arity(t2))} AND ${efsm2sal.guards2sal_num(Transition.Guards(t2), Nat.Nata(2))}) =>
+                  (input_sequence ! size?(i) = ${Code_Numeral.integer_of_nat(Transition.Arity(t1))} AND ${efsm2sal.guards2sal_num(Transition.Guards(t1), Nat.Nata(1))}))
                 )
               );""")
     val cmd = s"cd salfiles; sal-smc --assertion='${f}{${maxNum(e1, e2)}}!canStillTake'"
@@ -352,7 +352,7 @@ object Dirties {
     }
   }
 
-  def findDistinguishingGuard(
+  def findDistinguishingGuards(
     g1: (List[(List[Value.value], Map[Nat.nat, Option[Value.value]])]),
     g2: (List[(List[Value.value], Map[Nat.nat, Option[Value.value]])])): Option[(GExp.gexp[VName.vname], GExp.gexp[VName.vname])] = {
 
